

Ubaidullah Jamal

Time: 3:30

Difficulty: 3.5

Simplify Logarithms

$$\begin{aligned} \text{a) } & \log(x) + \log(y) - \log z \\ & \Rightarrow \log\left(\frac{xy}{z}\right) \end{aligned}$$

$$\begin{aligned} \text{b) } & 2\log(x) + 1 \\ & =, \log(x^2) + \log(e) \\ & =, \log(x^2 e) \end{aligned}$$

$$\begin{aligned} \text{c) } & \log(x) - 2\log(x) - 2 \\ & =, \log(x) - \log(e^2) \\ & =, \log\left(\frac{x}{e^2}\right) \end{aligned}$$

Sequences

$$a) u_n = 5 + 3n$$

$n=1$ $\Rightarrow u_1 = 8$	$n=2$ $\Rightarrow u_2 = 11$	$n=3$ $\Rightarrow u_3 = 14$
--------------------------------	---------------------------------	---------------------------------

This is an arithmetic sequence.

$$b) u_n = 3^n$$

$n=1$ $\Rightarrow u_1 = 3$	$n=2$ $u_2 = 9$	$n=3$ $u_3 = 27$
--------------------------------	--------------------	---------------------

Ratio:

$$\begin{aligned} r &= \frac{a_2}{a_1} = \frac{a_3}{a_2} \\ &= \frac{9}{3} = \frac{27}{9} \\ &= 3 = 3 \end{aligned}$$

This is a geometric sequence.

$$c) U_n = n \times 3^n$$

$n=1$ $U_1 = 1 \times 3^1$ $U_1 = 3$	$n=2$ $U_2 = 2 \times 3^2$ $U_2 = 18$	$n=3$ $U_3 = 3 \times 3^3$ $U_3 = 81$
--	---	---

This sequence is neither an arithmetic progression nor a geometric one.

Find the limit

$$a) U_n = 1 + \frac{1}{2}n$$

Sol:

In this sequence, the term $\left(\frac{1}{2}n = \frac{n}{2}\right)$ increases without bounds as $n \rightarrow \infty$, and as $n \rightarrow -\infty$, the term decreases ~~without bounds~~. As such, this sequence does not have a finite limit which we can call the general limit. ~~However,~~

$$b) U_n = \left(\frac{1}{2}\right)^n$$

Sol;

For this sequence, as n approaches $+\infty$, the sequence converges to 0; thus the limit ~~in this~~ from the right hand side tends to be 0.

From the left hand side, i.e., as n approaches $-\infty$, the sequence diverges to infinity. As such, this sequence does not have a general limit.

$$c) \lim_{x \rightarrow -4} \frac{x^2 + 5x + 4}{x^2 + 3x - 4}$$

$$\begin{aligned} \text{when } x &= -3.99 \\ \frac{(-3.99)^2 + 5(-3.99) + 4}{(-3.99)^2 + 3(-3.99) - 4} \\ &=, 0.599 \approx 0.6 \end{aligned}$$

$$\begin{aligned} \text{when } x &= -4.01 \\ \frac{(-4.01)^2 + 5(-4.01) + 4}{(-4.01)^2 + 3(-4.01) - 4} \\ &=, 0.6007 \approx 0.6 \end{aligned}$$

This seq. does have a limit as x approaches -4 which is ≈ 0.6

Determine convergence or divergence

$$a) \quad a_n = \frac{3+5n^2}{n+n^2}$$

div both num & den by n^2

$$a_n = \frac{3/n^2 + 5}{1/n + 1}$$

As $n \rightarrow +\infty$, both $3/n^2$ & $1/n$ tend to be 0,

$$a_n = \frac{0+5}{0+1} = 5$$

The same is true in case where $n \rightarrow -\infty$. As such, this seq. converges and the limit is 5.

$$b) \quad a_n = \frac{(-1)^{n-1} n}{n^2 + 1}$$

$$\text{when } n=1 \\ a_n = \frac{(-1)^{1-1}(1)}{(1)^2+1}$$

$$a_n = \frac{1}{2}$$

$$\text{when } n=2 \\ a_n = \frac{(-1)^{2-1}(2)}{(2)^2+1}$$

$$a_n = \frac{-2}{5}$$

when $n = -1$

$$a_n = \frac{(-1)^{-1-1}(-1)}{(-1)^2 + 1} = \frac{1/(-1)^2 \cdot (-1)}{1+1} = \frac{-1}{2}$$

As n approaches both +ve & -ve infinity, the sequence converges to 0, thus the limit, too, is zero.

Find more limits.

$$\lim_{x \rightarrow a} f(x) = -3, \lim_{x \rightarrow a} g(x) = 0, \lim_{x \rightarrow a} h(x) = 8$$

a) $\lim_{x \rightarrow a} [f(x) + h(x)]$

So,;

$$\begin{aligned} \Rightarrow \lim_{x \rightarrow a} [f(x) + h(x)] &= \lim_{x \rightarrow a} f(x) + \lim_{x \rightarrow a} h(x) \\ &= -3 + 8 \\ &= 5 \end{aligned}$$

The limit exists at 5 as $x \rightarrow a$.

b) $\lim_{x \rightarrow a} \frac{f(x)}{g(x)} = \frac{\lim_{x \rightarrow a} f(x)}{\lim_{x \rightarrow a} g(x)} = \frac{-3}{0} = \text{undefined}$

The limit does not exist as $x \rightarrow a$ as we get an undefined term & it violates the rule.

Also, the limit does not exist even if we approximate $g(x)$ as 0.001 or -0.001 as we get different results.

$$c) \lim_{x \rightarrow a} \frac{2f(x)}{h(x) - f(x)}$$

$$\neq \frac{\lim_{x \rightarrow a} f(x)}{\lim_{x \rightarrow a} h(x)} \neq \frac{\lim_{x \rightarrow a} f(x)}{\lim_{x \rightarrow a} f(x)}$$

$$= \frac{2 \lim_{x \rightarrow a} f(x)}{\lim_{x \rightarrow a} (h(x) - f(x))} = \frac{2 \lim_{x \rightarrow a} f(x)}{\lim_{x \rightarrow a} h(x) - \lim_{x \rightarrow a} f(x)}$$

$$= \frac{2(-3)}{8 - (-3)} = \frac{-6}{11}$$

The limit exists at $\frac{-6}{11}$

Check for discontinuities.

$$a) f(x) = \frac{9x^3 - x}{(x-1)(x+1)}$$

This function is discontinuous when $x=1$ or $x=-1$ as it leads to an undefined value.

$$b) f(x) = e^{-x^2}$$

This function is continuous as x approaches or moves away from 0 in either direction.

Find Finite Limits

$$a) \lim_{x \rightarrow 1} = \left[\frac{x^4 - 1}{x - 1} \right]$$

Sol:

$$\lim_{x \rightarrow 1} \left[\frac{(x^2+1)(x^2-1)}{x-1} \right]$$

$$\Rightarrow \lim_{x \rightarrow 1} \left[\frac{(x^2+1)(x+1)\cancel{(x-1)}}{\cancel{x-1}} \right]$$

~~as $x \rightarrow 1$~~

$$\lim_{x \rightarrow 1} (x^2+1)(x+1) = (1+1)(1+1) = 4$$

$$b) \lim_{x \rightarrow -4} \left[\frac{x^2 + 5x + 4}{x^2 + 3x - 4} \right]$$

Sol:

$$\lim_{x \rightarrow -4} \left[\frac{x^2 + 4x + x + 4}{x^2 + 4x - x - 4} \right]$$

$$\Rightarrow \lim_{x \rightarrow -4} \left[\frac{(x+4)(x+1)}{(x+4)(x-1)} \right]$$

$$\Rightarrow \lim_{x \rightarrow -4} \left[\frac{x+1}{x-1} \right] = \frac{-4+1}{-4-1} = \frac{-3}{-5} = \frac{3}{5}$$

Find Infinite Limits

$$a) \lim_{x \rightarrow \infty} \left[\frac{9x^2}{x^2+3} \right]$$

Applying L'Hopital's Rule ~~Rule~~

$$\lim_{x \rightarrow \infty} \left[\frac{9x^2}{x^2+3} \right] = \lim_{x \rightarrow \infty} \frac{18x}{2x} = \boxed{9}$$

$$b) \lim_{x \rightarrow \infty} \left[\frac{3^x}{x^3} \right]$$

Applying L'Hopital's Rule

$$\lim_{x \rightarrow \infty} \left[\frac{3^x}{x^3} \right] = \lim_{x \rightarrow \infty} \frac{3^x \log(3)}{3x^2}$$

Applying L'Hopital's law again,

$$\lim_{x \rightarrow \infty} \frac{3^x \log(3)}{3x^2} = \frac{3^x (\log(3))^2}{6x}$$

Applying L'Hopital's law again,

$$\lim_{x \rightarrow \infty} \frac{3^x (\log(3))^2}{6x} = \frac{3^x (\log(3))^3}{6}$$

As $x \rightarrow \infty$, so does 3^x or 3^∞ . As such the limit of $\frac{3^x}{x^3}$ as $x \rightarrow \infty$ is ∞ .

Assessing Continuity & Differentiability

$$a) f(x) = \begin{cases} +x^2, & x \geq 0 \\ -x^2, & x < 0 \end{cases}$$

So,;

For $x \geq 0$ and $x < 0$;

$$f(0) = 0^2 = 0$$

$$f(0) = -0^2 = 0$$

Continuous

Differentiating both x^2 & $-x^2$

$$2x \quad \& \quad -2x$$

$$2(0) \quad \& \quad -2(0)$$

$$0 = 0$$

Differentiable

$$b) f(x) = \begin{cases} x^3, & x \leq 1 \\ x, & x > 1 \end{cases}$$

For $x \leq 1$ & $x > 1$;

$$f(1) = x^3 = (1)^3 = 1$$

$$f(1) = x = 1$$

Continuous

Differentiating both x^3 & x

$$3x^2 \quad \& \quad 1$$

$$3(1)^2 \quad \& \quad 1$$

$$3 \neq 1$$

Not differentiable

Possible Derivatives

- A) Not possible - it is of a straight line
- B) Not possible - it is of a straight line
- C) C seems to be right as the line seems like that of a parabola & aligns with the zero.
- D) Seems wrong as the derivative seems both beneath & to the right of where the original graph of $f(x)$'s vertex is.

Calculate Derivatives.

$$\begin{aligned} \text{a) } f(x) &= 4x^3 + 2x^2 + 5x + 11 \\ \Rightarrow f'(x) &= 12x^2 + 4x + 5 \end{aligned}$$

$$\text{b) } y = \sqrt{30}$$

In this case, the derivative is 0 as it's a constant.

$$\begin{aligned} \text{c) } h(t) &= \log(qt+1) \\ &= \frac{1}{qt+1} (q) = \frac{q}{qt+1} \end{aligned}$$

$$\begin{aligned} \text{d) } f(x) &= \log(x^2 e^x) \\ &= \frac{1}{x^2 e^x} (2x e^x + x^2 e^x) \\ &= \frac{2x e^x + x^2 e^x}{x^2 e^x} \\ &= \frac{x e^x (2 + x)}{x^2 e^x} \\ &= \frac{2 + x}{x} \\ &= \frac{2}{x} + 1 \end{aligned}$$

$$\begin{aligned}
 e) \quad h(y) &= \left(\frac{1}{y^2} - \frac{3}{y^4} \right) (y + 5y^3) \\
 &= (y^{-2} - 3y^{-4}) (y + 5y^3) \\
 &= (-2y^{-3} + 12y^{-5}) (y + 5y^3) + \\
 &\quad \left(\frac{1}{y^2} - \frac{3}{y^4} \right) (15y^2 + 1) \\
 &= \left(-\frac{2}{y^3} + \frac{12}{y^5} \right) (y + 5y^3) + \left(\frac{1}{y^2} - \frac{3}{y^4} \right) (15y^2 + 1)
 \end{aligned}$$

$$\begin{aligned}
 f) \quad h(x) &= \frac{x}{\log(x)} \\
 &= \frac{1(\log(x)) - x(1/x)}{(\log(x))^2} \\
 &= \frac{\log(x) - 1}{(\log(x))^2}
 \end{aligned}$$

USE THE PRODUCT & QUOTIENT RULE

$$\begin{aligned}
 Q) f(x) &= \frac{x^2 - 2x}{x^4 + 6} \\
 &= \frac{(2x - 2)(x^4 + 6) - (x^2 - 2x)(4x^3)}{(x^4 + 6)^2} \\
 &= \frac{2x^5 + 12x - 2x^4 - 12 - 4x^5 + 8x^4}{(x^4 + 6)^2} \\
 &= \frac{-2x^5 + 6x^4 + 12x - 12}{x^8 + 12x^4 + 36}
 \end{aligned}$$

Using Product Rule.

$$\begin{aligned}
 f(x) &= (x^2 - 2x)(x^4 + 6)^{-1} \\
 &= (2x - 2)(x^4 + 6)^{-1} + (x^2 - 2x)(-1)(4x^3)(x^4 + 6)^{-2} \\
 &= \frac{(2x - 2)}{(x^4 + 6)} - \frac{4x^5 + 8x^4}{(x^4 + 6)^2} \\
 &= \frac{(2x - 2)(x^4 + 6) - 4x^5 + 8x^4}{(x^4 + 6)^2} \\
 &= \frac{2x^5 + 12x - 2x^4 - 12 - 4x^5 + 8x^4}{(x^4 + 6)^2} \\
 &= \frac{-2x^5 + 6x^4 + 12x - 12}{(x^4 + 6)^2}
 \end{aligned}$$

They are equivalent.

Composite Functions.

a) $q(x) = x^2 + 4$, $h(x) = 5x - 1$

For $q(h(x))$;

$$\begin{aligned} q(h(x)) &= q(5x - 1) = (5x - 1)^2 + 4 \\ &= 25x^2 - 10x + 5 \end{aligned}$$

Domain of $q(h(x)) = (-\infty, \infty)$

all real numbers

For $h(q(x)) = h(x^2 + 4) = 5(x^2 + 4) - 1$
 $= 5x^2 + 20 - 1$
 $= 5x^2 + 19$

Domain of $h(q(x)) = (-\infty, \infty)$

all real numbers

b) $q(x) = x^3$, $h(x) = (x - 1)(x + 1)$

For $q(h(x))$;

$$\begin{aligned} q(h(x)) &= q((x - 1)(x + 1)) = ((x - 1)(x + 1))^3 \\ &= (x^2 - 1)^3 \\ &= (x^2 - 1)^2 (x^2 - 1) \\ &= (x^4 - 2x^2 + 1)(x^2 - 1) \\ &= x^6 - 2x^4 + x^2 - x^4 + 2x^2 - 1 \\ &= x^6 - 3x^4 + 3x^2 - 1 \end{aligned}$$

Domain of $g(h(z)) = (-\infty, \infty)$
all real numbers

For $h(g(x))$;

$$h(g(x)) = h(x^3) = (x^3 - 1)(x^3 + 1) \\ = x^6 - 1$$

Domain of $g(h(z)) = (-\infty, \infty)$
all real numbers

CHAIN RULE

a) $g(x) = x^2 + 4$, $h(z) = 5z - 1$

Sol:

Derivative of $g(h(z))$:

• Directly

$$g(h(z)) = 25z^2 - 10z + 5$$

$$\frac{d}{dz} (g(h(z))) = 50z - 10$$

• Using chain rule

$$g'(h(z)) = 2(5z - 1)$$

$$h'(z) = 5$$

$$\frac{d}{dz} g(h(z)) = 2(5z - 1) \cdot 5 = 50z - 10$$

Derivative of $h(q(x))$

• Directly

$$h(q(x)) = 5x^2 + 9$$

$$\frac{d}{dx} (h(q(x))) = 10x$$

• Using Chain rule

$$h'(q(x)) = 5$$

$$q'(x) = 2x$$

$$\frac{d}{dx} h(q(x)) = 5 \cdot 2x = 10x$$

b) $q(x) = x^3$, $h(z) = (z-1)(z+1)$

Sol:

Derivative of $q(h(z))$

• Directly

$$q(h(z)) = z^6 - 3z^4 + 3z^2 - 1$$

$$\frac{d}{dz} (q(h(z))) = 6z^5 - 12z^3 + 6z$$

• Using Chain rule

$$q'(h(z)) = 3((z-1)(z+1))^2$$

$$h'(z) = 2z$$

$$\begin{aligned} \frac{d}{dz} q(h(z)) &= 3(z^2-1)^2 2z \\ &= 6z(z^4 - 2z^2 + 1) \\ &= 6z^5 - 12z^3 + 6z \end{aligned}$$

Derivative of $h(g(x))$.

• Directly

$$h(g(x)) = x^6 - 1$$

$$\frac{d}{dx} h(g(x)) = 6x^5 \leftarrow$$

• Using chain rule

$$h'(g(x)) = 2(x^3) \cdot \cancel{3x^2}$$

$$g'(x) = \cancel{3x^2} \cdot 3x^2$$

$$\frac{d}{dx} h(g(x)) = 2x^3 \cdot 3x^2 = 6x^5$$

c) $g(x) = 4x + 2$, $h(z) = \frac{1}{4}(z - 2)$

Solution.

For $g(h(z))$;

$$g'(h(z)) = 4$$

$$h'(z) = \frac{1}{4}$$

$$\frac{d}{dx} g(h(z)) = 4 \times \frac{1}{4} = 1$$

For $h(g(x))$;

$$h'(g(x)) = \frac{1}{4}$$

$$g'(x) = 4$$

$$\frac{d}{dx} h(g(x)) = \frac{1}{4} \times 4 = 1$$

$$b) f(x) = \begin{cases} x^3, & x \leq 1 \\ x, & x > 1 \end{cases}$$

For $x \leq 1$ & $x > 1$;

$$f(1) = x^3 = (1)^3 = 1$$

$$f(1) = x = 1$$

Continuous

Differentiating both x^3 & x

$$3x^2 \quad \& \quad 1$$

$$3(1)^2 \quad \& \quad 1$$

$$3 \neq 1$$

Not differentiable

Possible Derivatives

A) Not possible - it is of a straight line

B) Not possible - it is of a straight line

C) C seems to be right as the line seems like that of a parabola & aligns with the zero.

D) Seems wrong as the derivative seems both beneath & to the right of where the original graph $f(x)$'s vertex is.

The Other graph

Option B as it seems the best option for a derivative of a straight line.